progress learning lean4 syntax

Comp.lean
@@ -1,8 +1,117 @@
+-- TODO: port star from LoVe to Lean 4
+-- inductive star {α : Sort} (r : α → α → Prop) (a : α) : α → Prop where
+-- | refl _    : star a
+-- | tail {b c} : star b → r b c → star c
+
+-- attribute [refl] star.refl
+
+-- variables {α : Sort*} {r : α → α → Prop} {a b c d : α}
+
+-- @[trans] lemma trans (hab : star r a b) (hbc : star r b c) :
+--   star r a c :=
+-- begin
+--   induction' hbc,
+--   case refl {
+--     assumption },
+--   case tail : c d hbc hcd hac {
+--     exact (tail (hac hab)) hcd }
+-- end
+
+-- lemma single (hab : r a b) :
+--   star r a b :=
+-- refl.tail hab
+
+-- lemma head (hab : r a b) (hbc : star r b c) :
+--   star r a c :=
+-- begin
+--   induction' hbc,
+--   case refl {
+--     exact (tail refl) hab },
+--   case tail : c d hbc hcd hac {
+--     exact (tail (hac hab)) hcd }
+-- end
+
+-- lemma head_induction_on {α : Sort*} {r : α → α → Prop} {b : α}
+--   {P : ∀a : α, star r a b → Prop} {a : α} (h : star r a b)
+--   (refl : P b refl)
+--   (head : ∀{a c} (h' : r a c) (h : star r c b), P c h → P a (h.head h')) :
+--   P a h :=
+-- begin
+--   induction' h,
+--   case refl {
+--     exact refl },
+--   case tail : b c hab hbc ih {
+--     apply ih,
+--     show P b _, from
+--       head hbc _ refl,
+--     show ∀a a', r a a' → star r a' b → P a' _ → P a _, from
+--       assume a a' hab hbc, head hab _ }
+-- end
+
+-- lemma trans_induction_on {α : Sort*} {r : α → α → Prop}
+--     {p : ∀{a b : α}, star r a b → Prop} {a b : α} (h : star r a b)
+--     (ih₁ : ∀a, @p a a refl) (ih₂ : ∀{a b} (h : r a b), p (single h))
+--     (ih₃ : ∀{a b c} (h₁ : star r a b) (h₂ : star r b c), p h₁ →
+--        p h₂ → p (h₁.trans h₂)) :
+--   p h :=
+-- begin
+--   induction' h,
+--   case refl {
+--     exact ih₁ a },
+--   case tail : b c hab hbc ih {
+--     exact ih₃ hab (single hbc) (ih ih₁ @ih₂ @ih₃) (ih₂ hbc) }
+-- end
+
+-- lemma lift {β : Sort*} {s : β → β → Prop} (f : α → β)
+--   (h : ∀a b, r a b → s (f a) (f b)) (hab : star r a b) :
+--   star s (f a) (f b) :=
+-- hab.trans_induction_on
+--   (assume a, refl)
+--   (assume a b, single ∘ h _ _)
+--   (assume a b c _ _, trans)
+
+-- lemma mono {p : α → α → Prop} :
+--   (∀a b, r a b → p a b) → star r a b → star p a b :=
+-- lift id
+
+-- lemma star_star_eq :
+--   star (star r) = star r :=
+-- funext
+--   (assume a,
+--    funext
+--      (assume b,
+--       propext (iff.intro
+--         (assume h,
+--          begin
+--            induction' h,
+--            { refl },
+--            { transitivity;
+--                assumption }
+--          end)
+--         (star.mono (assume a b,
+--            single)))))
+
+
 
 
 def Val := Int
 
 def Stack := List Int
+
+def Stack.tail (stk : Stack) : Stack :=
+match stk with 
+| [] => []
+| (_ :: t) => t
+
+
+/-
+  Accomodating for Isabelle's support of head []
+  N.B. only problem of this could be if the stack is not controlled and the division is by zero
+-/
+def Stack.head (stk : Stack) : Int :=
+match stk with
+| [] => 0
+| (a::_) => a    
 
 def State : Type := String → Int
 
@@ -73,40 +182,116 @@ inductive Instr : Type where
 
 open Instr
 
-def iexec : Instr → Config → Config :=
-match 
-| (LOADI n) (i, s, stk) => (i + 1, s, n :: stk)
-| (LOAD v) (i, s, stk) => (i + 1, s, s v :: stk)
-| ADD (i, s, stk) => (i + 1, s, (stk.tail.head + stk.head) :: stk.tail.tail)
-| SUB (i, s, stk) => (i + 1, s, (stk.tail.head - stk.head) :: stk.tail.tail)
-| MUL (i, s, stk) => (i + 1, s, (stk.tail.head * stk.head) :: stk.tail.tail)
-| DIV (i, s, stk) => (i + 1, s, (stk.tail.head / stk.head) :: stk.tail.tail)
-| (STORE v) (i, s, stk) => (i + 1, s{v ↦ (stk.head)}, stk.tail)
-| (JMP n) (i, s, stk) => (i + 1 + n, s, stk)
-| (JMPLESS n) (i, s, stk) =>
-  if (stk.tail.head) < (stk.head)
-  then (i + 1 + n, s, stk.tail.tail)
-  else (i + 1, s, stk.tail.tail)
-| (JMPGE n) (i, s, stk) => 
-  if (stk.tail.head) ≥ (stk.head)
-  then (i + 1 + n, s, stk.tail.tail)
-  else (i + 1, s, stk.tail.tail)
-| NOP (i, s, stk) => (i, s, stk)
+def iexec (a : Instr) (c : Config) : Config :=
+match a with
+| (LOADI n) => (c.fst + 1, c.snd.fst, n :: c.snd.snd)
+| (LOAD v) => (c.fst + 1, c.snd.fst, c.snd.fst v :: c.snd.snd)
+| ADD => (c.fst + 1, c.snd.fst, (c.snd.snd.tail.head + c.snd.snd.head) :: c.snd.snd.tail.tail)
+| SUB => (c.fst + 1, c.snd.fst, (c.snd.snd.tail.head - c.snd.snd.head) :: c.snd.snd.tail.tail)
+| MUL => (c.fst + 1, c.snd.fst, (c.snd.snd.tail.head * c.snd.snd.head) :: c.snd.snd.tail.tail)
+| DIV => (c.fst + 1, c.snd.fst, (c.snd.snd.tail.head / c.snd.snd.head) :: c.snd.snd.tail.tail)
+| (STORE v) => (c.fst + 1, c.snd.fst{v ↦ (c.snd.snd.head)}, c.snd.snd.tail)
+| (JMP n) => (c.fst + 1 + n, c.snd.fst, c.snd.snd)
+| (JMPLESS n) =>
+  if (c.snd.snd.tail.head) < (c.snd.snd.head)
+  then (c.fst + 1 + n, c.snd.fst, c.snd.snd.tail.tail)
+  else (c.fst + 1, c.snd.fst, c.snd.snd.tail.tail)
+| (JMPGE n) => 
+  if (c.snd.snd.tail.head) ≥ (c.snd.snd.head)
+  then (c.fst + 1 + n, c.snd.fst, c.snd.snd.tail.tail)
+  else (c.fst + 1, c.snd.fst, c.snd.snd.tail.tail)
+| NOP => c
 
--- /- redefinition for ints rather than nat -/ 
--- def nth : (l : List Instr) (n : Int) :=
--- match l with
---   | (a :: l) n => if (n = 0) 
---     then a
---     else nth l (n - 1)
---   | list.nil n => NOP
+def nth (l : List Instr) (n : Int) : Instr :=
+  match l with
+  | [] => NOP
+  | (a :: l) => if (n = 0) 
+      then a
+      else nth l (n - 1)
 
--- def nth (as : List Instr) :
--- Fin (List.length as) → Instr :=
--- match as with
---   | (a :: tail) {val := 0, isLt := isLt} = a
---   | (head :: as) { val := Nat.succ i, isLt := h } =
---     nth as { val := i, isLt := (_ : Nat.succ i ≤ List.length as) }
+/- 
+  ## Single step execution
+  Execute one instruction
+  check if pc is in a valid location in the list 
+-/
+def exec1  (li : List Instr) (c : Config)  (c' : Config) : Prop := 
+( c' = iexec (nth li c.fst) c ∧ 0 ≤ c.fst ∧ c.fst < li.length)  
 
--- def nth (l : List Instr) (i : Int) : Instr :=
---   nth l i = if h : Instr then l[i] else NOP
+/-
+  ## Intro rule
+-/
+theorem exec1I (li : List Instr)
+  (h_eq: c' = iexec (nth li i) (i, s, stk))
+  (h_nneg : 0 ≤ i) 
+  (h_less : i < li.length):
+  exec1 li (i, s, stk) c' := by
+    simp [exec1]
+    simp [h_eq, h_nneg, h_less]
+  
+
+-- /- ## Multiple step execution -/
+-- def exec (li : List Instr) (c : Config) (c' : Config) : Prop :=
+-- star (exec1 li) c c'
+
+theorem iexec_shift_without_jmp {n : Int}  {i' : Int} {i : Int}:
+n + i' = n + i + 1 ↔ i' = i + 1 :=
+by
+  apply Iff.intro
+  . intro h_no_brackets
+    simp at h_no_brackets
+    sorry
+  . intro h
+    simp [h]
+    -- simp [Int.add_assoc]
+    sorry
+--   {
+--     intro h_no_brackets,
+--     have h_brackets: n + i' = n + (i + 1) := 
+--     begin
+--       simp [h_no_brackets],
+--       cc,
+--     end,
+--     apply int.add_left_cancel,
+--     apply h_brackets,
+--   },
+--   {
+--     intro h3,
+--     simp [h3],
+--     cc,
+--   },
+-- end
+
+theorem iexec_shift :
+((n + i',s',stk') = iexec instr (n + i, s, stk)) = ((i',s',stk') = iexec instr (i,s,stk)) := by
+cases instr
+case LOADI =>
+  simp [iexec]
+  sorry
+case LOAD =>
+  simp [iexec]
+  sorry
+case ADD =>
+  simp [iexec]
+  sorry
+case SUB =>
+  simp [iexec]
+  sorry
+case MUL =>
+  simp [iexec]
+  sorry
+case DIV =>
+  simp [iexec]
+  sorry
+case STORE =>
+  simp [iexec]
+  sorry
+case JMP => sorry
+case JMPLESS => sorry
+case JMPGE => sorry
+case NOP => 
+  simp [iexec]
+  sorry
+  -- apply iexec_shift_without_jmp
+  
+-- match instr with
+-- | (LOADI n) => 
